Lynx.lean
@@ -1,5 +1,4 @@
 import Lynx.Term
 import Lynx.Modules.Erlang
-import Lynx.Modules.Extensions
 import Lynx.Modules.Maps
 import Lynx.Tactic
